proof/invariant-abstract/KHeapPre_AI.thy
@@ -37,11 +37,6 @@ lemma dmo_return [simp]:
   by (simp add: do_machine_op_def select_f_def return_def gets_def get_def 
                 bind_def modify_def put_def)
 
-fun
-  non_arch_obj :: "kernel_object \<Rightarrow> bool" where
-  "non_arch_obj (ArchObj _) = False"
-  | "non_arch_obj _ = True"
-
 lemma get_object_sp:
   "\<lbrace>P\<rbrace> get_object p \<lbrace>\<lambda>r. P and ko_at r p\<rbrace>"
   apply (simp add: get_object_def)
@@ -49,32 +44,71 @@ lemma get_object_sp:
   apply (auto simp add: obj_at_def)
   done
 
+definition non_arch_obj :: "kernel_object \<Rightarrow> bool" where
+  "non_arch_obj \<equiv> \<lambda>ko. \<forall>ako. ko \<noteq> ArchObj ako"
 
+lemma non_arch_objs[intro]:
+  "non_arch_obj (Endpoint ep)"
+  "non_arch_obj (CNode sz cnode_contents)"
+  "non_arch_obj (TCB tcb)"
+  "non_arch_obj (Notification notification)"
+  by (auto simp add: non_arch_obj_def)
+
+definition arch_obj_pred :: "(kernel_object \<Rightarrow> bool) \<Rightarrow> bool" where
+  "arch_obj_pred P \<equiv>
+    \<forall>ko ko'. non_arch_obj ko \<longrightarrow> non_arch_obj ko' \<longrightarrow> 
+      P ko = P ko'"
+
+lemma arch_obj_predE:
+  "\<lbrakk>arch_obj_pred P; non_arch_obj ko; non_arch_obj ko'\<rbrakk> \<Longrightarrow> P ko = P ko'"
+  apply (unfold arch_obj_pred_def)
+  apply (erule allE[where ?x="ko"])
+  apply (erule allE[where ?x="ko'"])
+  by blast
+
+lemmas arch_obj_pred_defs = non_arch_obj_def arch_obj_pred_def
+
+lemma arch_obj_pred_a_type[intro, simp]: "arch_obj_pred (\<lambda>ko. a_type ko = AArch T)"
+  by (auto simp add: arch_obj_pred_defs a_type_def split: kernel_object.splits)
+
+lemma
+  arch_obj_pred_arch_obj_l[intro, simp]: "arch_obj_pred (\<lambda>ko. ArchObj ako = ko)" and
+  arch_obj_pred_arch_obj_r[intro, simp]: "arch_obj_pred (\<lambda>ko. ko = ArchObj ako)"
+  by (auto simp add: arch_obj_pred_defs)
+
+lemma arch_obj_pred_fun_lift: "arch_obj_pred (\<lambda>ko. F (arch_obj_fun_lift P N ko))"
+  by (simp add: arch_obj_pred_defs)
+
+lemmas arch_obj_pred_fun_lift_id[simp]
+  = arch_obj_pred_fun_lift[where F=id, simplified]
+
+lemmas arch_obj_pred_fun_lift_k[intro]
+  = arch_obj_pred_fun_lift[where F="K R" for R, simplified]
+
+lemmas arch_obj_pred_fun_lift_el[simp]
+  = arch_obj_pred_fun_lift[where F="\<lambda> S. x \<in> S" for x, simplified]
+
+lemma arch_obj_pred_const_conjI[intro]:
+  "arch_obj_pred P \<Longrightarrow>
+    arch_obj_pred P' \<Longrightarrow>
+    arch_obj_pred (\<lambda>ko. P ko \<and> P' ko)"
+  apply (simp only: arch_obj_pred_def)
+  apply blast
+  done
+
+lemma arch_obj_pred_fI:
+  "(\<And>x. arch_obj_pred (P x)) \<Longrightarrow> arch_obj_pred (\<lambda>ko. f (\<lambda>x :: 'a :: type. P x ko))"
+  apply (simp only: arch_obj_pred_def)
+  apply (intro allI impI)
+  apply (rule arg_cong[where f=f])
+  by blast
+
+declare
+  arch_obj_pred_fI[where f=All, intro]
+  arch_obj_pred_fI[where f=Ex, intro]
 
 locale arch_only_obj_pred =
   fixes P :: "kernel_object \<Rightarrow> bool"
-  assumes arch_only: "(\<And>ko. \<forall>ako. ko \<noteq> ArchObj ako \<Longrightarrow> \<not> P ko)" 
-begin
-
-lemma
-  obj_at_aobj_at: 
-  "obj_at P = aobj_at (\<lambda>ao. P (ArchObj ao))"
-  apply (insert arch_only)
-  apply (rule ext)+
-  apply (clarsimp simp add: aobj_at_def2 obj_at_def)
-  apply safe
-  apply (case_tac ko; simp)
-  apply (case_tac ko; simp)
-  done
-
-lemma
-  obj_at_lift:
-  assumes obj_at: "\<lbrace>aobj_at (\<lambda>ao. P (ArchObj ao)) p\<rbrace> f \<lbrace>\<lambda>r. aobj_at (\<lambda>ao. P (ArchObj ao)) p\<rbrace>"
-  shows "\<lbrace>obj_at P p\<rbrace> f \<lbrace>\<lambda>rv. obj_at P p\<rbrace>"
-  apply (simp add: obj_at_aobj_at)
-  apply (rule obj_at)
-  done
-
-end
+  assumes arch_only: "arch_obj_pred P" 
 
 end
