proof/invariant-abstract/ARM/ArchKHeap_AI.thy
@@ -16,16 +16,18 @@ context ARM begin
 
 sublocale 
   empty_table: arch_only_obj_pred "empty_table S" for S
-  by unfold_locales (simp add: empty_table_def)
+  by (unfold_locales, simp add: empty_table_def)
 
 sublocale
   vs_refs: arch_only_obj_pred "\<lambda>ko. x \<in> vs_refs ko" for S
-  apply unfold_locales
-  by (simp add: vs_refs_def)
+  by (unfold_locales, simp add: vs_refs_def del: vs_refs_arch_def)
 
+sublocale
+  vs_refs_pages: arch_only_obj_pred "\<lambda>ko. x \<in> vs_refs_pages ko" for S
+  by (unfold_locales, simp add: vs_refs_pages_def del: vs_refs_pages_arch_def)
 
 lemma pspace_in_kernel_window_atyp_lift_strong:
-  assumes atyp_inv: "\<And>P p T. \<lbrace>\<lambda>s. P (typ_at T p s)\<rbrace> f \<lbrace>\<lambda>rv s. P (typ_at T p s)\<rbrace>"
+  assumes atyp_inv: "\<And>P p T. \<lbrace> \<lambda>s. P (typ_at T p s) \<rbrace> f \<lbrace> \<lambda>rv s. P (typ_at T p s) \<rbrace>"
   assumes arch_inv: "\<And>P. \<lbrace>\<lambda>s. P (arm_kernel_vspace (arch_state s))\<rbrace> f \<lbrace>\<lambda>r s. P (arm_kernel_vspace (arch_state s))\<rbrace>"
   shows      "\<lbrace>\<lambda>s. pspace_in_kernel_window s\<rbrace> f \<lbrace>\<lambda>rv s. pspace_in_kernel_window s\<rbrace>"
   apply (simp add: pspace_in_kernel_window_def)
@@ -53,67 +55,58 @@ lemma pspace_in_kernel_window_atyp_lift:
   shows      "\<lbrace>\<lambda>s. pspace_in_kernel_window s\<rbrace> f \<lbrace>\<lambda>rv s. pspace_in_kernel_window s\<rbrace>"
   by (rule pspace_in_kernel_window_atyp_lift_strong[OF atyp_inv arch_inv])
 
-
 lemma cap_refs_in_kernel_window_arch_update[simp]:
   "arm_kernel_vspace (f (arch_state s)) = arm_kernel_vspace (arch_state s)
      \<Longrightarrow> cap_refs_in_kernel_window (arch_state_update f s) = cap_refs_in_kernel_window s"
   by (simp add: cap_refs_in_kernel_window_def not_kernel_window_arch_def)
-
 
 lemma
   ex_ko_at_def2: 
   "(\<exists>ko. ko_at ko p s \<and> P ko) = (obj_at P p s)"
   by (simp add: obj_at_def)
 
-lemma vs_lookup_aobj_at_lift:
-  assumes obj_at: "\<And>P P' p. \<lbrace>\<lambda>s. P (aobj_at P' p s)\<rbrace> f \<lbrace>\<lambda>r s. P (aobj_at P' p s)\<rbrace>"
+lemma vs_lookup_arch_obj_at_lift:
+  assumes obj_at: "\<And>P P' p. arch_obj_pred P' \<Longrightarrow>
+                             \<lbrace>\<lambda>s. P (obj_at P' p s)\<rbrace> f \<lbrace>\<lambda>r s. P (obj_at P' p s)\<rbrace>"
   assumes arch_state: "\<And>P. \<lbrace>\<lambda>s. P (arch_state s)\<rbrace> f \<lbrace>\<lambda>r s. P (arch_state s)\<rbrace>"
   shows "\<lbrace>\<lambda>s. P (vs_lookup s)\<rbrace> f \<lbrace>\<lambda>rv s. P (vs_lookup s)\<rbrace>"
-  apply (simp add: vs_lookup_def vs_lookup1_def vs_refs_def)
+  apply (simp add: vs_lookup_def vs_lookup1_def)
   apply (simp add: ex_ko_at_def2)
-  apply (subst arch_only_obj_pred.obj_at_aobj_at)
-  subgoal arch_only for \<dots> ko
-   apply unfold_locales
-   by (cases ko; simp)
-  apply (subst arch_only_obj_pred.obj_at_aobj_at[OF arch_only])
   apply (rule hoare_lift_Pf[where f="arch_state", OF _ arch_state])
-  apply (rule hoare_lift_Pf[where f="\<lambda>s rs p rs' p'. aobj_at (P' p rs rs' p') p s" for P'])
+  apply (rule hoare_lift_Pf[where f="\<lambda>s rs p rs' p'. obj_at (P' p rs rs' p') p s" for P'])
    apply (rule hoare_vcg_prop)
   apply (clarsimp simp add: valid_def)
   apply (erule_tac P=P in rsubst)
   apply (rule ext)+
   apply (erule use_valid, rule obj_at, simp)
-  done
+  by (auto simp: vs_refs.arch_only
+           intro!: arch_obj_pred_fI[where f=Ex])
 
-lemma vs_lookup_pages_aobj_at_lift:
-  assumes obj_at: "\<And>P P' p. \<lbrace>\<lambda>s. P (aobj_at P' p s)\<rbrace> f \<lbrace>\<lambda>r s. P (aobj_at P' p s)\<rbrace>"
+lemma vs_lookup_pages_arch_obj_at_lift:
+  assumes obj_at: "\<And>P P' p. arch_obj_pred P' \<Longrightarrow>
+                            \<lbrace>\<lambda>s. P (obj_at P' p s)\<rbrace> f \<lbrace>\<lambda>r s. P (obj_at P' p s)\<rbrace>"
   assumes arch_state: "\<And>P. \<lbrace>\<lambda>s. P (arch_state s)\<rbrace> f \<lbrace>\<lambda>r s. P (arch_state s)\<rbrace>"
   shows "\<lbrace>\<lambda>s. P (vs_lookup_pages s)\<rbrace> f \<lbrace>\<lambda>rv s. P (vs_lookup_pages s)\<rbrace>"
   apply (simp add: vs_lookup_pages_def vs_lookup_pages1_def)
   apply (simp add: ex_ko_at_def2)
-    apply (subst arch_only_obj_pred.obj_at_aobj_at)
-  subgoal arch_only for \<dots> ko
-   apply unfold_locales
-   by (cases ko; simp add: vs_refs_pages_def)
-  apply (subst arch_only_obj_pred.obj_at_aobj_at[OF arch_only])
   apply (rule hoare_lift_Pf[where f="arch_state", OF _ arch_state])
-  apply (rule hoare_lift_Pf[where f="\<lambda>s rs p rs' p'. aobj_at (P' p rs rs' p') p s" for P'])
+  apply (rule hoare_lift_Pf[where f="\<lambda>s rs p rs' p'. obj_at (P' p rs rs' p') p s" for P'])
    apply (rule hoare_vcg_prop)
   apply (clarsimp simp add: valid_def)
   apply (erule_tac P=P in rsubst)
   apply (rule ext)+
   apply (erule use_valid, rule obj_at, simp)
-  done
+  by (auto simp: vs_refs_pages.arch_only
+           intro!: arch_obj_pred_fI[where f=Ex])
 
 lemma valid_arch_objs_lift_weak:
-  assumes obj_at: "\<And>P P' p. \<lbrace>\<lambda>s. P (aobj_at P' p s)\<rbrace> f \<lbrace>\<lambda>r s. P (aobj_at P' p s)\<rbrace>"
+  assumes obj_at: "\<And>P P' p. arch_obj_pred P' \<Longrightarrow>
+                             \<lbrace>\<lambda>s. P (obj_at P' p s)\<rbrace> f \<lbrace>\<lambda>r s. P (obj_at P' p s)\<rbrace>"
   assumes arch_state: "\<And>P. \<lbrace>\<lambda>s. P (arch_state s)\<rbrace> f \<lbrace>\<lambda>r s. P (arch_state s)\<rbrace>"
   shows "\<lbrace>valid_arch_objs\<rbrace> f \<lbrace>\<lambda>_. valid_arch_objs\<rbrace>"
   apply (rule valid_arch_objs_lift)
-    apply (rule vs_lookup_aobj_at_lift)
-     apply (rule obj_at arch_state)+
-  apply (simp add: ko_at_ako[symmetric])
-  apply (rule obj_at)
+    apply (rule vs_lookup_arch_obj_at_lift)
+     apply (rule obj_at arch_state; simp)+
   done
 
 lemma set_object_neg_lookup:
@@ -160,7 +153,7 @@ lemma set_object_pt_not_vs_lookup_pages:
    \<lbrace>\<lambda>_ s. \<not>(ref \<unrhd> p') s\<rbrace>"
   apply (simp add: set_object_def)
   apply wp
-  apply (clarsimp simp: aobj_at_def)
+  apply (clarsimp simp: obj_at_def)
    apply (case_tac "(\<exists>\<unrhd>p) s")
    apply (erule notE)
    apply clarsimp
@@ -172,7 +165,7 @@ lemma set_object_pt_not_vs_lookup_pages:
    apply (drule vs_lookup_pages1D)
    apply (clarsimp simp: obj_at_def split:split_if_asm)
    apply (case_tac "pa=p")
-    apply (clarsimp simp: vs_refs_pages_def vs_refs_pages_arch_def graph_of_def)
+    apply (clarsimp simp: vs_refs_pages_def graph_of_def)
     apply (erule_tac x=ab in allE)
     apply (drule_tac R="vs_lookup_pages1 s" in rtranclD)
     apply clarsimp
@@ -220,15 +213,6 @@ lemma set_object_vs_lookup_pages:
   apply simp
   done
 
-lemma set_object_neg_ako:
-  "\<lbrace>not ako_at ko' p' and K (p = p' \<longrightarrow> ko \<noteq> ko')\<rbrace> 
-  set_object p (ArchObj ko) 
-  \<lbrace>\<lambda>_ s. \<not> ako_at ko' p' s\<rbrace>"
-  apply (simp add: set_object_def)
-  apply wp
-  apply (simp add: pred_neg_def aobj_at_def)
-  done
-
 lemma set_object_neg_ko:
   "\<lbrace>not ko_at ko' p' and K (p = p' \<longrightarrow> ko \<noteq> ko')\<rbrace> 
   set_object p ko 
@@ -237,7 +221,6 @@ lemma set_object_neg_ko:
   apply wp
   apply (simp add: pred_neg_def obj_at_def)
   done
-
 
 lemma set_object_typ_at:
   "\<lbrace>\<lambda>s. typ_at (a_type ko) p s \<and> P (typ_at T p' s)\<rbrace> 
@@ -250,13 +233,14 @@ lemma set_object_typ_at:
   done
 
 lemma set_object_atyp_at:
-  "\<lbrace>\<lambda>s. atyp_at (aa_type ko) p s \<and> P (atyp_at T p' s)\<rbrace> 
-  set_object p (ArchObj ko) \<lbrace>\<lambda>rv s. P (atyp_at T p' s)\<rbrace>"
+  "\<lbrace>\<lambda>s. typ_at (AArch (aa_type ako)) p s \<and> P (typ_at (AArch T) p' s)\<rbrace> 
+    set_object p (ArchObj ako)
+   \<lbrace>\<lambda>rv s. P (typ_at (AArch T) p' s)\<rbrace>"
   apply (simp add: set_object_def)
   apply wp
   apply clarsimp
   apply (erule rsubst [where P=P])
-  apply (clarsimp simp: aobj_at_def)
+  apply (clarsimp simp: obj_at_def a_type_aa_type)
   done
 
 lemma set_object_arch_objs:
@@ -271,7 +255,7 @@ lemma set_object_arch_objs:
   apply (subst imp_conv_disj)+
   apply (wp hoare_vcg_all_lift hoare_vcg_disj_lift set_object_neg_lookup set_object_neg_ko 
             valid_arch_obj_typ2 [where Q="typ_at (a_type ko) p"] set_object_typ_at
-         | simp add: atyp_at_def2)+
+         | simp)+
   apply (clarsimp simp: pred_neg_def obj_at_def)
   apply fastforce
   done
@@ -304,7 +288,7 @@ lemma valid_vs_lookup_lift:
   done
 
 
-lemma valid_table_caps_lift':
+lemma valid_table_caps_lift:
   assumes cap: "\<And>P. \<lbrace>\<lambda>s. P (caps_of_state s)\<rbrace> f \<lbrace>\<lambda>_ s. P (caps_of_state s)\<rbrace>"
   assumes pts: "\<And>P. \<lbrace>\<lambda>s. P (arm_global_pts (arch_state s))\<rbrace> f \<lbrace>\<lambda>_ s. P (arm_global_pts (arch_state s))\<rbrace>"
   assumes obj: "\<And>S p. \<lbrace>obj_at (empty_table S) p\<rbrace> f \<lbrace>\<lambda>rv. obj_at (empty_table S) p\<rbrace>"
@@ -315,9 +299,7 @@ lemma valid_table_caps_lift':
      apply (wp cap pts hoare_vcg_all_lift hoare_vcg_const_imp_lift obj)
   done
 
-lemmas valid_table_caps_lift = valid_table_caps_lift'[OF _ _ empty_table.obj_at_lift]
-
-lemma valid_arch_caps_lift':
+lemma valid_arch_caps_lift:
   assumes lookup: "\<And>P. \<lbrace>\<lambda>s. P (vs_lookup_pages s)\<rbrace> f \<lbrace>\<lambda>_ s. P (vs_lookup_pages s)\<rbrace>"
   assumes cap: "\<And>P. \<lbrace>\<lambda>s. P (caps_of_state s)\<rbrace> f \<lbrace>\<lambda>_ s. P (caps_of_state s)\<rbrace>"
   assumes pts: "\<And>P. \<lbrace>\<lambda>s. P (arm_global_pts (arch_state s))\<rbrace> f \<lbrace>\<lambda>_ s. P (arm_global_pts (arch_state s))\<rbrace>"
@@ -325,17 +307,15 @@ lemma valid_arch_caps_lift':
   shows "\<lbrace>valid_arch_caps\<rbrace> f \<lbrace>\<lambda>_. valid_arch_caps\<rbrace>"
   unfolding valid_arch_caps_def
   apply (rule hoare_pre)
-   apply (wp valid_vs_lookup_lift valid_table_caps_lift' lookup cap pts obj)
+   apply (wp valid_vs_lookup_lift valid_table_caps_lift lookup cap pts obj)
   apply simp
   done
-
-lemmas valid_arch_caps_lift = valid_arch_caps_lift'[OF _ _ _ empty_table.obj_at_lift]
 
 lemma valid_global_objs_lift':
   assumes pts: "\<And>P. \<lbrace>\<lambda>s. P (arm_global_pts (arch_state s))\<rbrace> f \<lbrace>\<lambda>_ s. P (arm_global_pts (arch_state s))\<rbrace>"
   assumes pd: "\<And>P. \<lbrace>\<lambda>s. P (arm_global_pd (arch_state s))\<rbrace> f \<lbrace>\<lambda>_ s. P (arm_global_pd (arch_state s))\<rbrace>"
   assumes obj: "\<And>p. \<lbrace>valid_ao_at p\<rbrace> f \<lbrace>\<lambda>rv. valid_ao_at p\<rbrace>"
-  assumes ko: "\<And>ao p. \<lbrace>ako_at ao p\<rbrace> f \<lbrace>\<lambda>_. ako_at ao p\<rbrace>"
+  assumes ko: "\<And>ako p. \<lbrace>ko_at (ArchObj ako) p\<rbrace> f \<lbrace>\<lambda>_. ko_at (ArchObj ako) p\<rbrace>"
   assumes emp: "\<And>pd S. 
        \<lbrace>\<lambda>s. (v \<longrightarrow> pd = arm_global_pd (arch_state s) \<and> S = set (arm_global_pts (arch_state s)) \<and> P s)
             \<and> obj_at (empty_table S) pd s\<rbrace>
@@ -345,18 +325,18 @@ lemma valid_global_objs_lift':
   apply (rule hoare_pre)
    apply (rule hoare_use_eq [where f="\<lambda>s. arm_global_pts (arch_state s)", OF pts])
    apply (rule hoare_use_eq [where f="\<lambda>s. arm_global_pd (arch_state s)", OF pd])
-   apply (wp obj ko[simplified ko_at_ako] emp hoare_vcg_const_Ball_lift hoare_ex_wp)
+   apply (wp obj ko emp hoare_vcg_const_Ball_lift hoare_ex_wp)
   apply clarsimp
   done
-
 
 lemmas valid_global_objs_lift
     = valid_global_objs_lift' [where v=False, simplified]
 
 lemma arch_lifts:
   assumes arch: "\<And>P. \<lbrace>\<lambda>s. P (arch_state s)\<rbrace> f \<lbrace>\<lambda>_ s. P (arch_state s)\<rbrace>"
-  assumes aobj_at: "\<And>P P' pd. \<lbrace>\<lambda>s. P (aobj_at P' pd s)\<rbrace> f \<lbrace>\<lambda>r s. P (aobj_at P' pd s)\<rbrace>"
-  shows 
+  assumes aobj_at: "\<And>P P' pd. arch_obj_pred P' \<Longrightarrow>
+    \<lbrace>\<lambda>s. P (obj_at P' pd s)\<rbrace> f \<lbrace>\<lambda>r s. P (obj_at P' pd s)\<rbrace>"
+  shows
   valid_global_pd_mappings_lift: 
     "\<lbrace>valid_global_pd_mappings\<rbrace> f \<lbrace>\<lambda>rv. valid_global_pd_mappings\<rbrace>" and
   valid_arch_caps_lift_weak: 
@@ -369,71 +349,81 @@ lemma arch_lifts:
   valid_kernel_mappings_lift:
     "\<lbrace>valid_kernel_mappings\<rbrace> f \<lbrace>\<lambda>rv. valid_kernel_mappings\<rbrace>"
   apply -
-  subgoal 
-  apply (simp add: valid_global_pd_mappings_def valid_pd_kernel_mappings_def obj_at_fun_lift)
+
+  subgoal
+  apply (simp add: valid_global_pd_mappings_def valid_pd_kernel_mappings_def
+              del: valid_pd_kernel_mappings_arch_def)
   apply (rule hoare_lift_Pf[where f="arch_state", OF _ arch])
   apply (rule_tac f="valid_pd_kernel_mappings_arch (arm_kernel_vspace x)" in hoare_lift_Pf)
-   apply (rule aobj_at)
+   apply (rule aobj_at; simp)
   apply (subst valid_pd_kernel_mappings_arch_def valid_pde_kernel_mappings_def)+
   apply (clarsimp simp add: valid_def)
   apply (erule_tac P=P in rsubst)
   apply (rule ext)
   apply (clarsimp intro!: iff_allI split: arch_kernel_obj.splits pde.splits)
-  apply (safe; clarsimp simp: valid_pt_kernel_mappings_def obj_at_fun_lift)
-     apply (erule (1) use_valid[OF _ aobj_at[where P="\<lambda>x. x"]])+
-   apply (rule classical, drule (1) use_valid[OF _ aobj_at[where P="\<lambda>x. \<not> x"]], simp)+
-   done
+  apply (safe; clarsimp simp add: valid_pt_kernel_mappings_def
+                        simp del: valid_pt_kernel_mappings_arch_def)
+     apply (erule use_valid[OF _ aobj_at[where P="\<lambda>x. x"]]; simp)+
+   by (rule classical,
+          drule use_valid[OF _ aobj_at[where P="\<lambda>x. \<not>x", OF arch_obj_pred_fun_lift_id]],
+          simp+)+
+
   subgoal
   apply (rule valid_arch_caps_lift[OF _ _ arch aobj_at])
-   apply (rule vs_lookup_pages_aobj_at_lift[OF aobj_at arch])
-  apply assumption
+    apply (rule vs_lookup_pages_arch_obj_at_lift[OF aobj_at arch], assumption+)
+  apply (rule empty_table.arch_only)
   done
+
   subgoal
   apply (rule valid_global_objs_lift)
       apply (wp arch)
     apply (simp add: valid_ao_at_def)
     apply (rule hoare_vcg_ex_lift)
     apply (rule hoare_vcg_conj_lift)
-     apply (wp aobj_at valid_arch_obj_atyp empty_table.obj_at_lift | simp add: ko_at_ako[symmetric])+
+     apply (wp aobj_at valid_arch_obj_typ | simp | rule empty_table.arch_only)+
   done
+
   subgoal
   apply (simp add: valid_asid_map_def)
   apply (rule hoare_lift_Pf[where f="arch_state", OF _ arch])
   apply (simp add: pd_at_asid_def)
-  by (rule vs_lookup_aobj_at_lift[OF aobj_at arch])
+  by (rule vs_lookup_arch_obj_at_lift[OF aobj_at arch])
+
   subgoal
   apply (simp add: valid_kernel_mappings_def)
   apply (rule hoare_lift_Pf[where f="arch_state", OF _ arch])
-  apply (simp add: valid_kernel_mappings_if_pd_def ran_def)
+  apply (simp add: valid_kernel_mappings_if_pd_def ran_def
+              del: valid_kernel_mappings_if_pd_arch_def)
   apply (rule hoare_vcg_all_lift)
   apply (case_tac "\<exists>ao. xa = ArchObj ao")
    apply (rule hoare_convert_imp)
     apply clarsimp
     apply (rule hoare_vcg_all_lift)
     subgoal for ao a
-    by (rule aobj_at[where P=Not and P'="\<lambda>x. x = ao", simplified aobj_at_def, simplified])
+    by (rule aobj_at[where P=Not and P'="\<lambda>x. x = ArchObj ao", simplified obj_at_def, simplified])
    apply clarsimp
    apply (case_tac ao; simp add: hoare_vcg_prop)
-  apply clarsimp
+  apply (clarsimp simp del: valid_kernel_mappings_if_pd_arch_def)
   apply (case_tac xa; simp add: hoare_vcg_prop)
   done
+
   done
 
 lemma equal_kernel_mappings_lift:
-  assumes aobj_at: "\<And>P P' pd. \<lbrace>\<lambda>s. P (aobj_at P' pd s)\<rbrace> f \<lbrace>\<lambda>r s. P (aobj_at P' pd s)\<rbrace>"
+  assumes aobj_at: "\<And>P P' pd. arch_obj_pred P' \<Longrightarrow>
+                               \<lbrace>\<lambda>s. P (obj_at P' pd s)\<rbrace> f \<lbrace>\<lambda>r s. P (obj_at P' pd s)\<rbrace>"
   shows "\<lbrace>equal_kernel_mappings\<rbrace> f \<lbrace>\<lambda>rv. equal_kernel_mappings\<rbrace>"
   apply (simp add: equal_kernel_mappings_def)
   apply (rule hoare_vcg_all_lift)+
   apply (rule hoare_convert_imp)
    apply simp
    apply (rule hoare_convert_imp)
-    apply (wp aobj_at)
+    apply (wp aobj_at[OF arch_obj_pred_arch_obj_l])
   done
-
 
 lemma valid_machine_state_lift:
   assumes memory: "\<And>P. \<lbrace>\<lambda>s. P (underlying_memory (machine_state s))\<rbrace> f \<lbrace>\<lambda>_ s. P (underlying_memory (machine_state s))\<rbrace>"
-  assumes aobj_at: "\<And>P' pd. \<lbrace>aobj_at P' pd\<rbrace> f \<lbrace>\<lambda>r s. aobj_at P' pd s\<rbrace>"
+  assumes aobj_at: "\<And>P' pd. arch_obj_pred P' \<Longrightarrow> \<lbrace>obj_at P' pd\<rbrace> f \<lbrace>\<lambda>r s. obj_at P' pd s\<rbrace>"
   shows "\<lbrace>valid_machine_state\<rbrace> f \<lbrace>\<lambda>_. valid_machine_state\<rbrace>"
   unfolding valid_machine_state_def in_user_frame_def
   apply (rule hoare_lift_Pf[where f="\<lambda>s. underlying_memory (machine_state s)", OF _ memory])
@@ -441,16 +431,16 @@ lemma valid_machine_state_lift:
   apply (rule hoare_vcg_disj_lift[OF _ hoare_vcg_prop])
   apply (rule hoare_vcg_ex_lift)
   subgoal for \<dots> sz
-   by (rule aobj_at[where P'="\<lambda>ao. ao = DataPage sz", simplified aobj_at_def[abs_def], simplified])
+   by (rule aobj_at[where P'="\<lambda>ao. ao = ArchObj (DataPage sz)",
+                    simplified obj_at_def[abs_def], simplified])
   done
-  
 
 lemma valid_ao_at_lift:
   assumes z: "\<And>P p T. \<lbrace>\<lambda>s. P (typ_at T p s)\<rbrace> f \<lbrace>\<lambda>rv s. P (typ_at T p s)\<rbrace>"
-      and y: "\<And>ao. \<lbrace>\<lambda>s. ako_at ao p s\<rbrace> f \<lbrace>\<lambda>rv s. ako_at ao p s\<rbrace>"
+      and y: "\<And>ao. \<lbrace>\<lambda>s. ko_at (ArchObj ao) p s\<rbrace> f \<lbrace>\<lambda>rv s. ko_at (ArchObj ao) p s\<rbrace>"
   shows      "\<lbrace>valid_ao_at p\<rbrace> f \<lbrace>\<lambda>rv. valid_ao_at p\<rbrace>"
   unfolding valid_ao_at_def
-  by (wp hoare_vcg_ex_lift y[simplified ko_at_ako] valid_arch_obj_typ z)
+  by (wp hoare_vcg_ex_lift y valid_arch_obj_typ z)
 
 
 lemmas set_object_v_ker_map
@@ -481,39 +471,39 @@ lemma set_object_asid_map:
 lemma set_object_equal_mappings:
   "\<lbrace>\<lambda>s. equal_kernel_mappings s
           \<and> (\<forall>pd. ko = ArchObj (PageDirectory pd)
-                \<longrightarrow> (\<forall>x pd'. ako_at (PageDirectory pd') x s
+                \<longrightarrow> (\<forall>x pd'. ko_at (ArchObj (PageDirectory pd')) x s
                          \<longrightarrow> (\<forall>w \<in> kernel_mapping_slots. pd w = pd' w)))\<rbrace>
      set_object p ko
    \<lbrace>\<lambda>rv. equal_kernel_mappings\<rbrace>"
   apply (simp add: set_object_def, wp)
-  apply (clarsimp simp: equal_kernel_mappings_def aobj_at_def
+  apply (clarsimp simp: equal_kernel_mappings_def obj_at_def
              split del: split_if)
   apply (simp split: split_if_asm)
   done
 
 lemma valid_global_pd_mappings_pres:
   "\<lbrakk> valid_global_pd_mappings s;
-     \<And>pd. ako_at (PageDirectory pd) (arm_global_pd (arch_state s)) s
-            \<Longrightarrow> ako_at (PageDirectory pd) (arm_global_pd (arch_state s)) s';
-     \<And>pt p. \<lbrakk> ako_at (PageTable pt) p s;
+     \<And>pd. ko_at (ArchObj (PageDirectory pd)) (arm_global_pd (arch_state s)) s
+            \<Longrightarrow> ko_at (ArchObj (PageDirectory pd)) (arm_global_pd (arch_state s)) s';
+     \<And>pt p. \<lbrakk> ko_at (ArchObj (PageTable pt)) p s;
                valid_global_objs s \<Longrightarrow> p \<in> set (arm_global_pts (arch_state s)) \<rbrakk>
-            \<Longrightarrow> ako_at (PageTable pt) p s';
+            \<Longrightarrow> ko_at (ArchObj (PageTable pt)) p s';
      arm_global_pd (arch_state s') = arm_global_pd (arch_state s);
      arm_kernel_vspace (arch_state s') = arm_kernel_vspace (arch_state s) \<rbrakk>
         \<Longrightarrow> valid_global_pd_mappings s'"
   apply atomize
-  apply (clarsimp simp: valid_global_pd_mappings_def aobj_at_def obj_at_def)
-  apply (clarsimp simp: valid_pd_kernel_mappings_def valid_pd_kernel_mappings_arch_def
-                 split: Structures_A.kernel_object.split_asm arch_kernel_obj.split_asm)
+  apply (clarsimp simp: valid_global_pd_mappings_def obj_at_def)
+  apply (clarsimp simp: valid_pd_kernel_mappings_def
+                 split: kernel_object.split_asm arch_kernel_obj.split_asm)
   apply (drule_tac x=x in spec)
-  apply (clarsimp simp: valid_pde_kernel_mappings_def valid_pd_kernel_mappings_arch_def obj_at_def
-                        valid_pt_kernel_mappings_def valid_pt_kernel_mappings_arch_def[abs_def]pde_ref_def
+  apply (clarsimp simp: valid_pde_kernel_mappings_def obj_at_def
+                        valid_pt_kernel_mappings_def pde_ref_def
                  split: Arch_Structs_A.ARM.pde.split_asm)
-  apply (simp split: Structures_A.kernel_object.split_asm
+  apply (simp split: kernel_object.split_asm
                      arch_kernel_obj.split_asm)
   apply (drule spec, drule spec, drule(1) mp)
   apply (drule mp)
-   apply (clarsimp simp: valid_global_objs_def obj_at_def empty_table_def empty_table_arch_def)
+   apply (clarsimp simp: valid_global_objs_def obj_at_def empty_table_def)
    apply (drule_tac x=x in spec)
    apply (simp add: pde_ref_def)[1]
   apply clarsimp
@@ -534,7 +524,7 @@ lemma set_object_global_pd_mappings:
   apply (simp add: set_object_def, wp)
   apply clarsimp
   apply (erule valid_global_pd_mappings_pres)
-     apply (clarsimp simp: aobj_at_def a_type_def aa_type_def global_refs_def)+
+     apply (clarsimp simp: obj_at_def a_type_def aa_type_def global_refs_def)+
   done
 
 
@@ -545,9 +535,9 @@ lemma valid_table_caps_ptD:
   apply (clarsimp simp: valid_table_caps_def simp del: split_paired_All)
   apply (erule allE)+
   apply (erule (1) impE)  
-  apply (clarsimp simp add: is_pt_cap_def cap_asid_def cap_asid_arch_def)
+  apply (clarsimp simp add: is_pt_cap_def cap_asid_def)
   apply (erule impE, rule refl)
-  apply (clarsimp simp: obj_at_def aobj_at_def empty_table_def empty_table_arch_def)
+  apply (clarsimp simp: obj_at_def empty_table_def)
   done
 
 lemma store_pde_pred_tcb_at:
